src/ExtractionHaskell/base_conversion.v
@@ -1,0 +1,4 @@
+Require Import Crypto.StandaloneHaskellMain.
+
+(*Redirect "/tmp/base_conversion.hs"*) Recursive Extraction BaseConversion.main.
+(* cat /tmp/base_conversion.hs.out | sed -f haskell.sed  > ../../base_conversion.hs *)
